coq_session

coq_session_new/tll_cren.v
@@ -1,6 +1,6 @@
 From mathcomp Require Import ssreflect ssrbool eqtype ssrnat seq.
 From Coq Require Import ssrfun Classical Utf8.
-Require Export AutosubstSsr ARS tll_ast sta_conf.
+Require Export AutosubstSsr ARS tll_classes sta_conf.
 
 Set Implicit Arguments.
 Unset Strict Implicit.
@@ -8,62 +8,52 @@ Unset Printing Implicit Defensive.
 
 Notation "( - n )" := (subn^~ n).
 
-Fixpoint term_cren (m : term) (ξ : cvar -> cvar) : term :=
-  match m with
-  (* core *)
-  | Var x => Var x
-  | Sort s => Sort s
-  | Pi0 A B s => Pi0 (term_cren A ξ) (term_cren B ξ) s
-  | Pi1 A B s => Pi1 (term_cren A ξ) (term_cren B ξ) s
-  | Lam0 A m s => Lam0 (term_cren A ξ) (term_cren m ξ) s
-  | Lam1 A m s => Lam1 (term_cren A ξ) (term_cren m ξ) s
-  | App0 m n => App0 (term_cren m ξ) (term_cren n ξ)
-  | App1 m n => App1 (term_cren m ξ) (term_cren n ξ)
-  | Sig0 A B s => Sig0 (term_cren A ξ) (term_cren B ξ) s
-  | Sig1 A B s => Sig1 (term_cren A ξ) (term_cren B ξ) s
-  | Pair0 m n s => Pair0 (term_cren m ξ) (term_cren n ξ) s
-  | Pair1 m n s => Pair1 (term_cren m ξ) (term_cren n ξ) s
-  | LetIn A m n =>
-      LetIn
-        (term_cren A ξ)
-        (term_cren m ξ)
-        (term_cren n ξ)
-  | Fix A m => Fix (term_cren A ξ) (term_cren m ξ)
-  (* data *)
-  | Unit => Unit
-  | II => II
-  | Bool => Bool
-  | TT => TT
-  | FF => FF
-  | Ifte A m n1 n2 =>
-      Ifte
-        (term_cren A ξ)
-        (term_cren m ξ)
-        (term_cren n1 ξ)
-        (term_cren n2 ξ)
-  (* monadic *)
-  | IO A => IO (term_cren A ξ)
-  | Return m => Return (term_cren m ξ)
-  | Bind m n => Bind (term_cren m ξ) (term_cren n ξ)
-  (* session *)
-  | Proto => Proto
-  | Stop => Stop
-  | Act0 r A B => Act0 r (term_cren A ξ) (term_cren B ξ)
-  | Act1 r A B => Act1 r (term_cren A ξ) (term_cren B ξ)
-  | Ch r A => Ch r (term_cren A ξ)
-  | CVar x => CVar (ξ x)
-  | Fork A m => Fork (term_cren A ξ) (term_cren m ξ)
-  | Recv0 m => Recv0 (term_cren m ξ)
-  | Recv1 m => Recv1 (term_cren m ξ)
-  | Send0 m => Send0 (term_cren m ξ)
-  | Send1 m => Send1 (term_cren m ξ)
-  | Close m => Close (term_cren m ξ)
-  | Wait m => Wait (term_cren m ξ)
-  | Box => Box
-  end.
+#[global] Instance CRename_term : CRename term :=
+  fix dummy (ξ : cvar -> cvar) (m : term) : term :=
+    let term_cren := @cren term dummy in
+    match m with
+    (* core *)
+    | Var x => Var x
+    | Sort s => Sort s
+    | Pi0 A B s => Pi0 (term_cren ξ A) (term_cren ξ B) s
+    | Pi1 A B s => Pi1 (term_cren ξ A) (term_cren ξ B) s
+    | Lam0 A m s => Lam0 (term_cren ξ A) (term_cren ξ m) s
+    | Lam1 A m s => Lam1 (term_cren ξ A) (term_cren ξ m) s
+    | App0 m n => App0 (term_cren ξ m) (term_cren ξ n)
+    | App1 m n => App1 (term_cren ξ m) (term_cren ξ n)
+    | Sig0 A B s => Sig0 (term_cren ξ A) (term_cren ξ B) s
+    | Sig1 A B s => Sig1 (term_cren ξ A) (term_cren ξ B) s
+    | Pair0 m n s => Pair0 (term_cren ξ m) (term_cren ξ n) s
+    | Pair1 m n s => Pair1 (term_cren ξ m) (term_cren ξ n) s
+    | LetIn A m n => LetIn (term_cren ξ A) (term_cren ξ m) (term_cren ξ n)
+    | Fix A m => Fix (term_cren ξ A) (term_cren ξ m)
+    (* data *)
+    | Unit => Unit | II => II | Bool => Bool | TT => TT | FF => FF
+    | Ifte A m n1 n2 =>
+      Ifte (term_cren ξ A) (term_cren ξ m) (term_cren ξ n1) (term_cren ξ n2)
+    (* monadic *)
+    | IO A => IO (term_cren ξ A)
+    | Return m => Return (term_cren ξ m)
+    | Bind m n => Bind (term_cren ξ m) (term_cren ξ n)
+    (* session *)
+    | Proto => Proto
+    | Stop => Stop
+    | Act0 r A B => Act0 r (term_cren ξ A) (term_cren ξ B)
+    | Act1 r A B => Act1 r (term_cren ξ A) (term_cren ξ B)
+    | Ch r A => Ch r (term_cren ξ A)
+    | CVar x => (fun x => CVar (ξ x)) x
+    | Fork A m => Fork (term_cren ξ A) (term_cren ξ m)
+    | Recv0 m => Recv0 (term_cren ξ m)
+    | Recv1 m => Recv1 (term_cren ξ m)
+    | Send0 m => Send0 (term_cren ξ m)
+    | Send1 m => Send1 (term_cren ξ m)
+    | Close m => Close (term_cren ξ m)
+    | Wait m => Wait (term_cren ξ m)
+    | Box => Box
+    end.
 
 Lemma term_cren_ren m ξ ξ' :
-  term_cren m.[ren ξ] ξ' = (term_cren m ξ').[ren ξ].
+  cren ξ' m.[ren ξ] = (cren ξ' m).[ren ξ].
 Proof with eauto.
   elim: m ξ ξ'...
   { move=>A ihA B ihB s ξ ξ'. asimpl.
@@ -113,7 +103,7 @@ Proof with eauto.
   { move=>m ihm ξ ξ'. asimpl. rewrite ihm... }
 Qed.
 
-Lemma term_cren_id m : term_cren m id = m.
+Lemma term_cren_id m : cren id m = m.
 Proof with eauto.
   elim: m=>//=...
   { move=>A ihA B ihB s. rewrite ihA. by rewrite ihB. }
@@ -146,7 +136,7 @@ Proof with eauto.
 Qed.
 
 Lemma term_cren_comp ξ1 ξ2 m :
-  term_cren m (ξ1 >>> ξ2) = term_cren (term_cren m ξ1) ξ2.
+  cren (ξ1 >>> ξ2) m = cren ξ2 (cren ξ1 m).
 Proof with eauto.
   elim: m ξ1 ξ2=>//=.
   { move=>A ihA B ihB s ξ1 ξ2. rewrite ihA. by rewrite ihB. }
@@ -179,10 +169,10 @@ Proof with eauto.
 Qed.
 
 Definition cren_subst_agree (σ σ' : var -> term) ξ :=
-  forall x, σ' x = term_cren (σ x) ξ.
+  forall x, σ' x = cren ξ (σ x).
 
 Lemma term_cren_subst1 n ξ :
-  cren_subst_agree (n .: ids) (term_cren n ξ .: ids) ξ.
+  cren_subst_agree (n .: ids) (cren ξ n .: ids) ξ.
 Proof with eauto.
   move=>x.
   elim: x n ξ.
@@ -191,7 +181,7 @@ Proof with eauto.
 Qed.
 
 Lemma term_cren_subst2 n1 n2 ξ :
-  cren_subst_agree (n1 .: n2 .: ids) (term_cren n1 ξ .: term_cren n2 ξ .: ids) ξ.
+  cren_subst_agree (n1 .: n2 .: ids) (cren ξ n1 .: cren ξ n2 .: ids) ξ.
 Proof with eauto.
   move=>x.
   elim: x n1 n2 ξ.
@@ -223,22 +213,16 @@ Proof.
 Qed.
 
 Lemma term_cren_subst m σ σ' ξ :
-  cren_subst_agree σ σ' ξ -> term_cren m.[σ] ξ = (term_cren m ξ).[σ'].
+  cren_subst_agree σ σ' ξ -> cren ξ m.[σ] = (cren ξ m).[σ'].
 Proof.
   elim: m σ σ' ξ.
   all: solve[intros; asimpl; f_equal; eauto using term_cren_subst_up].
 Qed.
 
 Lemma term_cren_beta1 m n ξ :
-  term_cren m.[n/] ξ = (term_cren m ξ).[term_cren n ξ/].
-Proof.
-  apply: term_cren_subst.
-  apply: term_cren_subst1.
-Qed.
+  cren ξ m.[n/] = (cren ξ m).[cren ξ n/].
+Proof. apply: term_cren_subst. apply: term_cren_subst1. Qed.
 
 Lemma term_cren_beta2 m n1 n2 ξ :
-  term_cren m.[n1,n2/] ξ = (term_cren m ξ).[term_cren n1 ξ,term_cren n2 ξ/].
-Proof.
-  apply: term_cren_subst.
-  apply: term_cren_subst2.
-Qed.
+  cren ξ m.[n1,n2/] = (cren ξ m).[cren ξ n1,cren ξ n2/].
+Proof. apply: term_cren_subst. apply: term_cren_subst2. Qed.
