coq_session_new/tllc_csubst.v
@@ -6,28 +6,30 @@ Set Implicit Arguments.
 Unset Strict Implicit.
 Unset Printing Implicit Defensive.
 
-Fixpoint proc_csubst (p : proc) (σ : cvar -> term) :=
-  match p with
-  | Exp m => Exp (term_csubst m σ)
-  | Par p q => Par (proc_csubst p σ) (proc_csubst q σ)
-  | Nu p => Nu (proc_csubst p (upp (upp σ)))
-  end.
+#[global] Instance CSubst_proc : CSubst proc :=
+  fix dummy (σ : cvar -> term) (p : proc) : proc :=
+    let proc_csubst := @csubst proc dummy in
+    match p with
+    | Exp m => Exp (csubst σ m)
+    | Par p q => Par (proc_csubst σ p) (proc_csubst σ q)
+    | Nu p => Nu (proc_csubst (cup (cup σ)) p)
+    end.
 
-Lemma proc_csubst_cids p : proc_csubst p cids = p. 
+Lemma proc_csubst_cids p : csubst cids p = p. 
 Proof with eauto.
   elim: p=>//=...
   { move=>m. rewrite term_csubst_cids... }
   { move=>p ihp q ihq. autorew... }
-  { move=>p e. rewrite! upp_cids. rewrite e... }
+  { move=>p e. rewrite! cup_cids. rewrite e... }
 Qed.
 
 Lemma proc_csubst_comp p σ1 σ2 :
-  proc_csubst (proc_csubst p σ1) σ2 = proc_csubst p (σ1 >>> term_csubst^~ σ2).
+  csubst σ2 (csubst σ1 p) = csubst (σ1 >>> csubst σ2) p.
 Proof.
   elim: p σ1 σ2=>//=.
   { move=>m σ1 σ2. by rewrite term_csubst_comp. }
   { move=>p ihp q ihq σ1 σ2. by autorew. }
   { move=>p ihp σ1 σ2. f_equal.
     rewrite ihp. f_equal.
-    apply: (term_uppn_comp σ1 σ2 2). }
+    apply: (term_cupn_comp σ1 σ2 2). }
 Qed.
