coq_session_new/eproc_cren.v
@@ -7,12 +7,12 @@ Unset Strict Implicit.
 Unset Printing Implicit Defensive.
 
 Lemma eproc_crename Θ Θ' p p' ξ :
-  Θ ⊢ p ~ p' -> dyn_ctx_cren ξ Θ Θ' -> Θ' ⊢ proc_cren p ξ ~ proc_cren p' ξ.
+  Θ ⊢ p ~ p' -> dyn_ctx_cren ξ Θ Θ' -> Θ' ⊢ cren ξ p ~ cren ξ p'.
 Proof with eauto.
   move=>er. elim: er Θ' ξ=>{Θ p p'}.
   { move=>Θ m m' tym Θ' ξ agr/=.
     constructor.
-    replace (IO Unit) with (term_cren (IO Unit) ξ) by eauto.
+    replace (IO Unit) with (cren ξ (IO Unit)) by eauto.
     apply: era_crename... }
   { move=>Θ1 Θ2 Θ p p' q q' mrg typ ihp tyq ihq Θ' ξ agr/=.
     have[Θ1'[Θ2'[mrg'[agr1 agr2]]]]:=dyn_ctx_cren_merge agr mrg.
@@ -26,19 +26,19 @@ Proof with eauto.
     rewrite<-term_cren_comp in agr0.
     have e:((+1) >>> upren ξ) = (ξ >>> (+1)) by autosubst.
     rewrite e in agr0.
-    have{}e:(term_cren A (ξ >>> (+1)))= term_cren (term_cren A ξ) (+1).
+    have{}e:(cren (ξ >>> (+1)) A)= cren (+1) (cren ξ A).
     by rewrite<-term_cren_comp.
     rewrite e in agr0.
     apply: agr0. }
 Qed.
 
-Lemma eproc_cstrengthen Θ p p' : _: Θ ⊢ proc_cren p (+1) ~ proc_cren p' (+1) -> Θ ⊢ p ~ p'.
+Lemma eproc_cstrengthen Θ p p' : _: Θ ⊢ cren (+1) p ~ cren (+1) p' -> Θ ⊢ p ~ p'.
 Proof.
   move=>ty.
   have e:((+1) >>> (-1)) = id.
   { f_ext. move=>x. asimpl. fold subn. lia. }
-  replace p with (proc_cren (proc_cren p (+1)) ((-1) >>> id)).
-  replace p' with (proc_cren (proc_cren p' (+1)) ((-1) >>> id)).
+  replace p with (cren ((-1) >>> id) (cren (+1) p)).
+  replace p' with (cren ((-1) >>> id) (cren (+1) p')).
   apply: eproc_crename.
   apply: ty.
   repeat constructor.
@@ -50,7 +50,7 @@ Proof.
   by rewrite proc_cren_id.
 Qed.
 
-Lemma eproc_cweaken Θ p p' : Θ ⊢ p ~ p' -> _: Θ ⊢ proc_cren p (+1) ~ proc_cren p' (+1). 
+Lemma eproc_cweaken Θ p p' : Θ ⊢ p ~ p' -> _: Θ ⊢ cren (+1) p ~ cren (+1) p'. 
 Proof with eauto.
   move=>ty.
   apply: eproc_crename...
@@ -59,9 +59,9 @@ Proof with eauto.
 Qed.
 
 Lemma eproc_cren_inv Θ p x ξ :
-  Θ ⊢ proc_cren p ξ ~ x -> exists p', x = proc_cren p' ξ. 
+  Θ ⊢ cren ξ p ~ x -> exists p', x = cren ξ p'. 
 Proof with eauto.
-  move e:(proc_cren p ξ)=>n er. elim: er p ξ e=>{Θ x n}.
+  move e:(cren ξ p)=>n er. elim: er p ξ e=>{Θ x n}.
   { move=>Θ m m' erm p ξ e. destruct p; inv e.
     have[m1 e]:=era_cren_inv erm. subst. by exists ⟨ m1 ⟩. }
   { move=>Θ1 Θ2 Θ p p' q q' mrg erp ihp erq ihq p0 ξ e.
