coq_session_new/eproc_sr.v
@@ -8,7 +8,7 @@ Unset Printing Implicit Defensive.
 
 Lemma eproc_exch_type Θ p p' :
   Θ ⊢ Nu (Nu p) ~ Nu (Nu p') →
-  Θ ⊢ Nu (Nu (proc_csubst p exch)) ~ Nu (Nu (proc_csubst p' exch)).
+  Θ ⊢ Nu (Nu (csubst exch p)) ~ Nu (Nu (csubst exch p')).
 Proof with eauto using dyn_wf, key.
   move=>ty. inv ty. inv H3.
   have wf:=eproc_type_wf H4. inv wf. inv H1. inv H2. inv H1.
@@ -16,15 +16,15 @@ Proof with eauto using dyn_wf, key.
   econstructor... econstructor...
   apply: eproc_csubstitution. apply: H4.
   have mrg:
-    Ch (~~ r2) (term_cren A (+1)) :L Ch r2 A :L _: Ch r0 A0 :L Θ ∘
-    _: _: Ch (~~ r0) (term_cren A0 (+1)) :L _: Θ0 =>
-    Ch (~~ r2) (term_cren A (+1)) :L Ch r2 A :L
-    Ch (~~ r0) (term_cren A0 (+1)) :L Ch r0 A0 :L Θ.
+    Ch (~~ r2) (cren (+1) A) :L Ch r2 A :L _: Ch r0 A0 :L Θ ∘
+    _: _: Ch (~~ r0) (cren (+1) A0) :L _: Θ0 =>
+    Ch (~~ r2) (cren (+1) A) :L Ch r2 A :L
+    Ch (~~ r0) (cren (+1) A0) :L Ch r0 A0 :L Θ.
   { repeat constructor. apply: merge_sym... }
   econstructor...
   2:{ have//=js:
-        dyn_just (_: _: Ch (~~ r0) (term_cren A0 (+1)) :L _: Θ0) 2
-        (term_cren (term_cren (term_cren (Ch (~~ r0) (term_cren A0 (+1))) (+1)) (+1)) (+1)).
+        dyn_just (_: _: Ch (~~ r0) (cren (+1) A0) :L _: Θ0) 2
+        (cren (+1) (cren (+1) (cren (+1) (Ch (~~ r0) (cren (+1) A0))))).
       { repeat constructor... }
       apply: dyn_conv.
       2:{ constructor... repeat apply: sta_crename... }
@@ -33,14 +33,14 @@ Proof with eauto using dyn_wf, key.
       apply: conv_sym. apply: sta_cren_conv0. eauto.
       constructor... }
   have{}mrg:
-    Ch (~~ r2) (term_cren A (+1)) :L Ch r2 A :L _: _: Θ ∘
+    Ch (~~ r2) (cren (+1) A) :L Ch r2 A :L _: _: Θ ∘
     _: _: _: Ch r0 A0 :L Θ0 =>
-    Ch (~~ r2) (term_cren A (+1)) :L Ch r2 A :L _: Ch r0 A0 :L Θ.
+    Ch (~~ r2) (cren (+1) A) :L Ch r2 A :L _: Ch r0 A0 :L Θ.
   { repeat constructor. apply: merge_sym... }
   econstructor...
   2:{ have//=js:
         dyn_just (_: _: _: Ch r0 A0 :L Θ0) 3
-        (term_cren (term_cren (term_cren (term_cren (Ch r0 A0) (+1)) (+1)) (+1)) (+1)).
+        (cren (+1) (cren (+1) (cren (+1) (cren (+1) (Ch r0 A0))))).
       { repeat constructor... }
       apply: dyn_conv.
       2:{ constructor... repeat apply: sta_crename... }
@@ -49,13 +49,13 @@ Proof with eauto using dyn_wf, key.
       constructor... }
   have{}mrg:
     _: Ch r2 A :L _: _: Θ ∘
-    Ch (~~ r2) (term_cren A (+1)) :L _: _: _: Θ0 =>
-    Ch (~~ r2) (term_cren A (+1)) :L Ch r2 A :L _: _: Θ.
+    Ch (~~ r2) (cren (+1) A) :L _: _: _: Θ0 =>
+    Ch (~~ r2) (cren (+1) A) :L Ch r2 A :L _: _: Θ.
   { repeat constructor. apply: merge_sym... }
   econstructor...
   2:{ have//=js:
-        dyn_just (Ch (~~ r2) (term_cren A (+1)) :L _: _: _: Θ0) 0
-        (term_cren (Ch (~~ r2) (term_cren A (+1))) (+1)).
+        dyn_just (Ch (~~ r2) (cren (+1) A) :L _: _: _: Θ0) 0
+        (cren (+1) (Ch (~~ r2) (cren (+1) A))).
       { repeat constructor... }
       apply: dyn_conv.
       2:{ constructor... apply: sta_crename... }
@@ -65,15 +65,15 @@ Proof with eauto using dyn_wf, key.
   { repeat constructor. apply: merge_sym... }
   econstructor...
   2:{ have//=js:
-        dyn_just (_: Ch r2 A :L _: _: Θ0) 1 (term_cren (term_cren (Ch r2 A) (+1)) (+1)).
+        dyn_just (_: Ch r2 A :L _: _: Θ0) 1 (cren (+1) (cren (+1) (Ch r2 A))).
       { repeat constructor... }
       apply: dyn_conv.
       2:{ constructor... apply: sta_crename... }
       asimpl. apply: sta_conv_ch. repeat apply: sta_cren_conv0...
       constructor... }
   have->: (fun x => CVar x.+4) =
-          (cids >>> term_cren^~(+1) >>> term_cren^~(+1)
-                >>> term_cren^~(+1) >>> term_cren^~(+1)).
+          (cids >>> cren (+1) >>> cren (+1)
+                >>> cren (+1) >>> cren (+1)).
   { f_ext. move=>x. by simpl. }
   repeat constructor...
 Qed.
@@ -94,14 +94,14 @@ Proof with eauto using era_type, eproc_type, proc_congr0.
     econstructor. apply: merge_sym.
     all: eauto. }
   { move=>p q Θ p' er. inv er. inv H3.
-    exists (ν.(p' ∣ proc_cren q' (+2))).
+    exists (ν.(p' ∣ cren (+2) q')).
     constructor.
     move: H4. move e:(~~r2)=>r1 erp.
     econstructor. apply: (esym e).
     econstructor.
     2:{ apply: erp. }
-    2:{ replace (proc_cren q (+2)) with (proc_cren (proc_cren q (+1)) (+1)).
-        replace (proc_cren q' (+2)) with (proc_cren (proc_cren q' (+1)) (+1)).
+    2:{ replace (cren (+2) q) with (cren (+1) (cren (+1) q)).
+        replace (cren (+2) q') with (cren (+1) (cren (+1) q')).
         apply: eproc_cweaken.
         apply: eproc_cweaken.
         apply: H5.
@@ -109,7 +109,7 @@ Proof with eauto using era_type, eproc_type, proc_congr0.
         rewrite<-proc_cren_comp. by asimpl. }
     repeat constructor... }
   { move=>p Θ p' ty. have ty0:=ty. inv ty. inv H2.
-    exists (Nu (Nu (proc_csubst p' exch))). constructor.
+    exists (Nu (Nu (csubst exch p'))). constructor.
     apply: eproc_exch_type... }
   { move=>p p' q q' cgr1 ih1 cgr2 ih2 Θ p0 er. inv er.
     have[p1 cgr3 erp]:=ih1 _ _ H3.
@@ -145,10 +145,10 @@ Proof with eauto using era_type, eproc_type, proc_congr0.
     econstructor... }
   { move=>p q Θ q' er. inv er. inv H2. inv H1; inv H3.
     { have[q0 e]:=eproc_cren_inv H6. subst.
-      replace (proc_cren q (+2))
-        with (proc_cren (proc_cren q (+1)) (+1)) in H6.
-      replace (proc_cren q0 (+2))
-        with (proc_cren (proc_cren q0 (+1)) (+1)) in H6.
+      replace (cren (+2) q)
+        with (cren (+1) (cren (+1) q)) in H6.
+      replace (cren (+2) q0)
+        with (cren (+1) (cren (+1) q0)) in H6.
       have erq:=eproc_cstrengthen (eproc_cstrengthen H6).
       exists (ν.p'0 ∣ q0).
       constructor.
@@ -157,28 +157,28 @@ Proof with eauto using era_type, eproc_type, proc_congr0.
       rewrite<-proc_cren_comp. by asimpl. }
     { have[q0 e]:=eproc_cren_inv H6. subst.
       have:=eproc_occurs_iren H6 iren1.
-      have[->_]:proc_occurs 1 (proc_cren q (+2)) = 1 ∧
-               proc_occurs 1 (proc_cren q0 (+2)) = 1.
+      have[->_]:proc_occurs 1 (cren (+2) q) = 1 ∧
+               proc_occurs 1 (cren (+2) q0) = 1.
       apply: eproc_type_occurs1...
       repeat constructor.
       by move=>[]. }
     { have[q0 e]:=eproc_cren_inv H6. subst.
       have:=eproc_occurs_iren H6 iren0.
-      have[->_]:proc_occurs 0 (proc_cren q (+2)) = 1 ∧
-               proc_occurs 0 (proc_cren q0 (+2)) = 1.
+      have[->_]:proc_occurs 0 (cren (+2) q) = 1 ∧
+               proc_occurs 0 (cren (+2) q0) = 1.
       apply: eproc_type_occurs1...
       repeat constructor.
       by move=>[]. }
     { have[q0 e]:=eproc_cren_inv H6. subst.
       have:=eproc_occurs_iren H6 iren0.
-      have[->_]:proc_occurs 0 (proc_cren q (+2)) = 1 ∧
-               proc_occurs 0 (proc_cren q0 (+2)) = 1.
+      have[->_]:proc_occurs 0 (cren (+2) q) = 1 ∧
+               proc_occurs 0 (cren (+2) q0) = 1.
       apply: eproc_type_occurs1...
       repeat constructor.
       by move=>[]. } }
   { move=>p Θ q' ty. have ty0:=ty. inv ty. inv H2.
-    exists (Nu (Nu (proc_csubst p'0 exch))).
-    replace (Nu (Nu p'0)) with (Nu (Nu (proc_csubst (proc_csubst p'0 exch) exch))).
+    exists (Nu (Nu (csubst exch p'0))).
+    replace (Nu (Nu p'0)) with (Nu (Nu (csubst exch (csubst exch p'0)))).
     constructor.
     rewrite proc_csubst_comp.
     rewrite exch_invo. rewrite proc_csubst_cids...
@@ -235,8 +235,8 @@ Proof with eauto using merge, merge_sym, sta_type, era_type.
     have[Θ1[Θ2[Δ1[Δ2[A0[s[mrg1[mrg2[tyF/=tyn]]]]]]]]]:=
       era_bind_inv ty. inv mrg2. inv mrg1. inv H2.
     have[_[tym/io_inj eq2]]:=era_fork_inv tyF.
-    have mrg0: Ch (~~ true) (term_cren A (+1)) :L _: Δ3 ∘ _: Ch true A :L Δ0 =>
-           Ch (~~ true) (term_cren A (+1)) :L Ch true A :L Θ.
+    have mrg0: Ch (~~ true) (cren (+1) A) :L _: Δ3 ∘ _: Ch true A :L Δ0 =>
+           Ch (~~ true) (cren (+1) A) :L Ch true A :L Θ.
     { econstructor. econstructor. apply: merge_sym... }
     econstructor. 2:{ apply: proc_step_fork... }
     econstructor...
@@ -245,8 +245,8 @@ Proof with eauto using merge, merge_sym, sta_type, era_type.
       have wf:=era_type_wf tym. inv wf.
       have wf:=era_type_proc_wf tyn. inv wf. inv H0.
       have[Θ0[emp mrg1]]:=proc_wf_empty H1.
-      have{}mrg1: _: _: Δ3 ∘ Ch (~~ true) (term_cren A (+1)) :L _: Θ0 =>
-            Ch (~~ true) (term_cren A (+1)) :L _: Δ3...
+      have{}mrg1: _: _: Δ3 ∘ Ch (~~ true) (cren (+1) A) :L _: Θ0 =>
+            Ch (~~ true) (cren (+1) A) :L _: Δ3...
       have[tyA _]:=sta_ch_inv H7.
       have[x eq3 eq4]:=church_rosser eq2.
       have tyx1:=sta_prd H5 eq3.
@@ -255,8 +255,8 @@ Proof with eauto using merge, merge_sym, sta_type, era_type.
       have tyIO:(A0 :: nil) ⊢ (IO Unit).[ren (+1)] : (Sort L).[ren (+1)].
       { apply: sta_weaken... }
       have/=js: dyn_just
-                  (Ch (~~ true) (term_cren A (+1)) :L _: Θ0) 0
-                  (term_cren (Ch (~~ true) (term_cren A (+1))) (+1)).
+                  (Ch (~~ true) (cren (+1) A) :L _: Θ0) 0
+                  (cren (+1) (Ch (~~ true) (cren (+1) A))).
       { constructor. constructor... }
       rewrite<-term_cren_comp in js. asimpl in js.
       econstructor.
@@ -268,8 +268,8 @@ Proof with eauto using merge, merge_sym, sta_type, era_type.
       replace (IO Unit) with (IO Unit.[ren (+1)]) by eauto.
       apply: era_conv.
       apply: conv_sym...
-      replace (Ch false (term_cren A (+2)))
-        with (Ch false (term_cren A (+2)).[ren (+0)])
+      replace (Ch false (cren (+2) A))
+        with (Ch false (cren (+2) A).[ren (+0)])
         by autosubst.
       repeat constructor...
       apply: H5. }
@@ -288,12 +288,12 @@ Proof with eauto using merge, merge_sym, sta_type, era_type.
       apply: era_esubst1...
       apply: key_impure.
       apply: key_impure.
-      replace (Ch true (term_cren A (+2)))
-        with (Ch true (term_cren A (+2)).[ren (+0)])
+      replace (Ch true (cren (+2) A))
+        with (Ch true (cren (+2) A).[ren (+0)])
         by autosubst.
       repeat constructor...
-      replace (Ch true (term_cren A (+2)))
-        with (term_cren (Ch true (term_cren A (+1))) (+1)).
+      replace (Ch true (cren (+2) A))
+        with (cren (+1) (Ch true (cren (+1) A))).
       repeat constructor...
       simpl. rewrite<-term_cren_comp.
       by autosubst. } }
@@ -375,11 +375,11 @@ Proof with eauto using merge, merge_sym, sta_type, era_type.
               apply: convR _.
               apply: conv_sym...
               simpl.
-              replace (term_cren B2.[m/] (+2))
-                with (term_cren B2.[m/] (+2)).[ren (+0)] by autosubst.
+              replace (cren (+2) B2.[m/])
+                with (cren (+2) B2.[m/]).[ren (+0)] by autosubst.
               repeat constructor.
-              replace (Ch (~~ r) (term_cren B2.[m/] (+2)))
-                with (term_cren (Ch (~~ r) (term_cren B2.[m/] (+1))) (+1)).
+              replace (Ch (~~ r) (cren (+2) B2.[m/]))
+                with (cren (+1) (Ch (~~ r) (cren (+1) B2.[m/]))).
               2:{ simpl. rewrite<-term_cren_comp. autosubst. }
               eapply dyn_just_O.
               apply: dyn_empty_n...
@@ -418,12 +418,12 @@ Proof with eauto using merge, merge_sym, sta_type, era_type.
       eauto.
       rewrite term_cren_beta1.
       simpl.
-      replace (term_cren B2 (+2)).[term_cren m (+2)/]
-        with (term_cren B2 (+2)).[term_cren m (+2)/].[ren (+0)] by autosubst.
+      replace (cren (+2) B2).[cren (+2) m/]
+        with (cren (+2) B2).[cren (+2) m/].[ren (+0)] by autosubst.
       repeat constructor.
       rewrite<-term_cren_beta1.
-      replace (Ch r (term_cren B2.[m/] (+2)))
-        with (term_cren (Ch r (term_cren B2.[m/] (+1))) (+1)).
+      replace (Ch r (cren (+2) B2.[m/]))
+        with (cren (+1) (Ch r (cren (+1) B2.[m/]))).
       repeat constructor...
       simpl. rewrite<-term_cren_comp. asimpl...
       rewrite<-term_cren_beta1.
@@ -543,11 +543,11 @@ Proof with eauto using merge, merge_sym, sta_type, era_type.
               apply: conv_sym...
               2:{ eauto. }
               simpl.
-              replace (Ch r (term_cren B4.[m/] (+2)))
-                with (Ch r (term_cren B4.[m/] (+2))).[ren (+0)] by autosubst.
+              replace (Ch r (cren (+2) B4.[m/]))
+                with (Ch r (cren (+2) B4.[m/])).[ren (+0)] by autosubst.
               econstructor...
-              replace (Ch r (term_cren B4.[m/] (+2)))
-                with (term_cren (term_cren (Ch r B4.[m/]) (+1)) (+1)).
+              replace (Ch r (cren (+2) B4.[m/]))
+                with (cren (+1) (cren (+1) (Ch r B4.[m/]))).
               constructor.
               constructor...
               rewrite<-term_cren_comp. asimpl...
@@ -589,11 +589,11 @@ Proof with eauto using merge, merge_sym, sta_type, era_type.
           apply: sta_conv_subst.
           apply: conv_sym...
           asimpl.
-          replace (Ch (~~r) (term_cren B4.[m/] (+2)))
-            with (Ch (~~r) (term_cren B4.[m/] (+2))).[ren (+0)] by autosubst.
+          replace (Ch (~~r) (cren (+2) B4.[m/]))
+            with (Ch (~~r) (cren (+2) B4.[m/])).[ren (+0)] by autosubst.
           econstructor...
-          replace (Ch (~~r) (term_cren B4.[m/] (+2)))
-            with (term_cren (term_cren (Ch (~~r) B4.[m/]) (+1)) (+1)).
+          replace (Ch (~~r) (cren (+2) B4.[m/]))
+            with (cren (+1) (cren (+1) (Ch (~~r) B4.[m/]))).
           constructor.
           apply: dyn_empty_n...
           rewrite<-term_cren_comp...
@@ -706,13 +706,13 @@ Proof with eauto using merge, merge_sym, sta_type, era_type.
               apply: conv_sym...
               2:{ apply: H9. }
               simpl.
-              replace (term_cren B4.[v/] (+2))
-                with (term_cren B4.[v/] (+2)).[ren (+0)] by autosubst.
+              replace (cren (+2) B4.[v/])
+                with (cren (+2) B4.[v/]).[ren (+0)] by autosubst.
               constructor...
               2:{ constructor. }
               2:{ apply: sta_crename... }
-              replace (Ch (~~ r5) (term_cren B4.[v/] (+2)))
-                with (term_cren (Ch (~~ r5) (term_cren B4.[v/] (+1))) (+1)).
+              replace (Ch (~~ r5) (cren (+2) B4.[v/]))
+                with (cren (+1) (Ch (~~ r5) (cren (+1) B4.[v/]))).
               constructor.
               apply: dyn_empty_n...
               simpl. rewrite<-term_cren_comp. by asimpl. }
@@ -739,7 +739,7 @@ Proof with eauto using merge, merge_sym, sta_type, era_type.
                   eauto. }
               2:{ econstructor... }
               2:{ asimpl.
-                  have eq:term_cren (Ch r5 B4.[v/]) (+2) === Ch r5 B2.[v/].
+                  have eq:cren (+2) (Ch r5 B4.[v/]) === Ch r5 B2.[v/].
                   { apply: conv_trans.
                     apply: sta_cren_conv0.
                     apply: sta_conv_ch.
@@ -750,11 +750,11 @@ Proof with eauto using merge, merge_sym, sta_type, era_type.
                   apply: eq.
                   2:{ constructor... }
                   simpl.
-                  replace (Ch r5 (term_cren B4.[v/] (+2)))
-                    with (Ch r5 (term_cren B4.[v/] (+2))).[ren (+0)] by autosubst.
+                  replace (Ch r5 (cren (+2) B4.[v/]))
+                    with (Ch r5 (cren (+2) B4.[v/])).[ren (+0)] by autosubst.
                   constructor...
-                  replace (Ch r5 (term_cren B4.[v/] (+2)))
-                    with (term_cren (term_cren (Ch r5 B4.[v/]) (+1)) (+1)).
+                  replace (Ch r5 (cren (+2) B4.[v/]))
+                    with (cren (+1) (cren (+1) (Ch r5 B4.[v/]))).
                   constructor.
                   constructor.
                   eauto.
@@ -891,13 +891,13 @@ Proof with eauto using merge, merge_sym, sta_type, era_type.
               apply: conv_sym...
               2:{ eauto. }
               simpl.
-              replace (Ch r (term_cren B5.[v/] (+2)))
-                with (Ch r (term_cren B5.[v/] (+2))).[ren (+0)] by autosubst.
+              replace (Ch r (cren (+2) B5.[v/]))
+                with (Ch r (cren (+2) B5.[v/])).[ren (+0)] by autosubst.
               constructor.
               2:{ constructor. }
               2:{ constructor. }
-              replace (Ch r (term_cren B5.[v/] (+2)))
-                with (term_cren (term_cren (Ch r B5.[v/]) (+1)) (+1)).
+              replace (Ch r (cren (+2) B5.[v/]))
+                with (cren (+1) (cren (+1) (Ch r B5.[v/]))).
               constructor.
               constructor.
               eauto.
@@ -931,14 +931,14 @@ Proof with eauto using merge, merge_sym, sta_type, era_type.
                   apply: eqB5.
                   2:{ constructor... }
                   simpl.
-                  replace (Ch (~~r) (term_cren B5.[v/] (+2)))
-                    with (Ch (~~r) (term_cren B5.[v/] (+2))).[ren (+0)] by autosubst.
+                  replace (Ch (~~r) (cren (+2) B5.[v/]))
+                    with (Ch (~~r) (cren (+2) B5.[v/])).[ren (+0)] by autosubst.
                   constructor.
                   2:{ constructor. }
                   2:{ constructor. }
                   2:{ apply: sta_crename... }
-                  replace (Ch (~~r) (term_cren B5.[v/] (+2)))
-                    with (term_cren (term_cren (Ch (~~r) B5.[v/]) (+1)) (+1)).
+                  replace (Ch (~~r) (cren (+2) B5.[v/]))
+                    with (cren (+1) (cren (+1) (Ch (~~r) B5.[v/]))).
                   constructor.
                   apply: dyn_empty_n...
                   rewrite<-term_cren_comp. asimpl... }
@@ -1022,20 +1022,20 @@ Proof with eauto using merge, merge_sym, sta_type, era_type.
       econstructor. 2:{ apply: proc_step_end... }
       econstructor...
       { constructor.
-        replace (IO Unit) with (term_cren (IO Unit) (-2)) by eauto.
-        replace (Bind (Return II) (term_cren m (-2)))
-          with (term_cren (Bind (Return II) m) (-2)) by eauto.
-        replace (Bind (Return II) (term_cren m1' (-2)))
-          with (term_cren (Bind (Return II) m1') (-2)) by eauto.
+        replace (IO Unit) with (cren (-2) (IO Unit)) by eauto.
+        replace (Bind (Return II) (cren (-2) m))
+          with (cren (-2) (Bind (Return II) m)) by eauto.
+        replace (Bind (Return II) (cren (-2) m1'))
+          with (cren (-2) (Bind (Return II) m1')) by eauto.
         rewrite e.
         apply: era_crename...
         repeat constructor. }
       { constructor.
-        replace (IO Unit) with (term_cren (IO Unit) (-2)) by eauto.
-        replace (Bind (Return II) (term_cren n (-2)))
-          with (term_cren (Bind (Return II) n) (-2)) by eauto.
-        replace (Bind (Return II) (term_cren n' (-2)))
-          with (term_cren (Bind (Return II) n') (-2)) by eauto.
+        replace (IO Unit) with (cren (-2) (IO Unit)) by eauto.
+        replace (Bind (Return II) (cren (-2) n))
+          with (cren (-2) (Bind (Return II) n)) by eauto.
+        replace (Bind (Return II) (cren (-2) n'))
+          with (cren (-2) (Bind (Return II) n')) by eauto.
         rewrite e.
         apply: era_crename...
         repeat constructor. } }
@@ -1122,20 +1122,20 @@ Proof with eauto using merge, merge_sym, sta_type, era_type.
       econstructor. 2:{ apply: proc_step_endi... }
       econstructor...
       { constructor.
-        replace (IO Unit) with (term_cren (IO Unit) (-2)) by eauto.
-        replace (Bind (Return II) (term_cren m (-2)))
-          with (term_cren (Bind (Return II) m) (-2)) by eauto.
-        replace (Bind (Return II) (term_cren m1' (-2)))
-          with (term_cren (Bind (Return II) m1') (-2)) by eauto.
+        replace (IO Unit) with (cren (-2) (IO Unit)) by eauto.
+        replace (Bind (Return II) (cren (-2) m))
+          with (cren (-2) (Bind (Return II) m)) by eauto.
+        replace (Bind (Return II) (cren (-2) m1'))
+          with (cren (-2) (Bind (Return II) m1')) by eauto.
         rewrite e.
         apply: era_crename...
         repeat constructor. }
       { constructor.
-        replace (IO Unit) with (term_cren (IO Unit) (-2)) by eauto.
-        replace (Bind (Return II) (term_cren n (-2)))
-          with (term_cren (Bind (Return II) n) (-2)) by eauto.
-        replace (Bind (Return II) (term_cren n' (-2)))
-          with (term_cren (Bind (Return II) n') (-2)) by eauto.
+        replace (IO Unit) with (cren (-2) (IO Unit)) by eauto.
+        replace (Bind (Return II) (cren (-2) n))
+          with (cren (-2) (Bind (Return II) n)) by eauto.
+        replace (Bind (Return II) (cren (-2) n'))
+          with (cren (-2) (Bind (Return II) n')) by eauto.
         rewrite e.
         apply: era_crename...
         repeat constructor. } }
