coq_session_new/proc_cren.v
@@ -7,12 +7,12 @@ Unset Strict Implicit.
 Unset Printing Implicit Defensive.
 
 Lemma proc_crename Θ Θ' p ξ :
-  Θ ⊢ p -> dyn_ctx_cren ξ Θ Θ' -> Θ' ⊢ proc_cren p ξ.
+  Θ ⊢ p -> dyn_ctx_cren ξ Θ Θ' -> Θ' ⊢ cren ξ p.
 Proof with eauto.
   move=>ty. elim: ty Θ' ξ=>{Θ p}.
   { move=>Θ m tym Θ' ξ agr/=.
     constructor.
-    replace (IO Unit) with (term_cren (IO Unit) ξ) by eauto.
+    replace (IO Unit) with (cren ξ (IO Unit)) by eauto.
     apply: dyn_crename... }
   { move=>Θ1 Θ2 Θ p q mrg typ ihp tyq ihq Θ' ξ agr/=.
     have[Θ1'[Θ2'[mrg'[agr1 agr2]]]]:=dyn_ctx_cren_merge agr mrg.
@@ -26,18 +26,18 @@ Proof with eauto.
     rewrite<-term_cren_comp in agr0.
     have e:((+1) >>> upren ξ) = (ξ >>> (+1)) by autosubst.
     rewrite e in agr0.
-    have{}e:(term_cren A (ξ >>> (+1)))= term_cren (term_cren A ξ) (+1).
+    have{}e:(cren (ξ >>> (+1)) A)= cren (+1) (cren ξ A).
     by rewrite<-term_cren_comp.
     rewrite e in agr0.
     apply: agr0. }
 Qed.
 
-Lemma proc_cstrengthen Θ p : _: Θ ⊢ proc_cren p (+1) -> Θ ⊢ p.
+Lemma proc_cstrengthen Θ p : _: Θ ⊢ cren (+1) p -> Θ ⊢ p.
 Proof.
   move=>ty.
   have e:((+1) >>> (-1)) = id.
   { f_ext. move=>x. asimpl. fold subn. lia. }
-  replace p with (proc_cren (proc_cren p (+1)) ((-1) >>> id)).
+  replace p with (cren ((-1) >>> id) (cren (+1) p)).
   apply: proc_crename.
   apply: ty.
   constructor.
@@ -48,7 +48,7 @@ Proof.
   by rewrite proc_cren_id.
 Qed.
 
-Lemma proc_cweaken Θ p : Θ ⊢ p -> _: Θ ⊢ proc_cren p (+1). 
+Lemma proc_cweaken Θ p : Θ ⊢ p -> _: Θ ⊢ cren (+1) p. 
 Proof with eauto.
   move=>ty.
   apply: proc_crename...
