coq_session_new/proc_csubst.v
@@ -7,7 +7,7 @@ Unset Strict Implicit.
 Unset Printing Implicit Defensive.
 
 Lemma proc_csubstitution Θ2 Θ1 p σ :
-  Θ2 ⊢ p -> Θ1 ⊩ σ ⫣ Θ2 -> Θ1 ⊢ proc_csubst p σ. 
+  Θ2 ⊢ p -> Θ1 ⊩ σ ⫣ Θ2 -> Θ1 ⊢ csubst σ p. 
 Proof with eauto.
   move=>ty. elim: ty Θ1 σ=>{Θ2 p}.
   { move=>Θ m tym Θ1 σ agr. constructor.
