coq_session_new/proc_type.v
@@ -19,7 +19,7 @@ Inductive proc_type : dyn_ctx -> proc -> Prop :=
   Θ ⊢ p ∣ q
 | proc_scope Θ p r1 r2 A :
   r1 = ~~r2 ->
-  Ch r1 (term_cren A (+1)) :L Ch r2 A :L Θ ⊢ p ->
+  Ch r1 (cren (+1) A) :L Ch r2 A :L Θ ⊢ p ->
   Θ ⊢ ν.p
 where "Θ ⊢ p" := (proc_type Θ p).
 
@@ -98,5 +98,3 @@ Proof with eauto using merge, dyn_empty.
   move=>Θ r A wf[Θ'[emp mrg]]tyA. exists (_: Θ')...
   move=>Θ wf[Θ'[emp mrg]]. exists (_: Θ')...
 Qed.
-
-         
