coq_session_new/tll_classes.v
@@ -1,0 +1,8 @@
+Require Import AutosubstSsr ARS tll_ast.
+
+Class CRename (A : Type) := cren : (cvar -> cvar) -> A -> A.
+Class CSubst (A : Type)  := csubst : (cvar -> term) -> A -> A.
+
+Arguments cren {_ _} xi !m /.
+Arguments csubst {_ _} sigma !m /.
+
